concurrency/bst_conc.v
@@ -12,7 +12,7 @@ Module Info.
   Definition bitsize := 32.
   Definition big_endian := false.
   Definition source_file := "bst_conc.c"%string.
-  Definition normalized := false.
+  Definition normalized := true.
 End Info.
 
 Definition ___builtin_ais_annot : ident := 9%positive.
@@ -67,66 +67,69 @@ Definition ___compcert_va_composite : ident := 26%positive.
 Definition ___compcert_va_float64 : ident := 25%positive.
 Definition ___compcert_va_int32 : ident := 23%positive.
 Definition ___compcert_va_int64 : ident := 24%positive.
-Definition ___stringlit_1 : ident := 102%positive.
-Definition ___stringlit_2 : ident := 103%positive.
-Definition ___stringlit_3 : ident := 104%positive.
-Definition ___stringlit_4 : ident := 105%positive.
-Definition ___stringlit_5 : ident := 106%positive.
-Definition __l : ident := 90%positive.
-Definition _acquire : ident := 66%positive.
-Definition _b : ident := 76%positive.
-Definition _delete : ident := 101%positive.
-Definition _free : ident := 62%positive.
-Definition _freelock : ident := 65%positive.
-Definition _insert : ident := 85%positive.
+Definition ___stringlit_1 : ident := 105%positive.
+Definition ___stringlit_2 : ident := 106%positive.
+Definition ___stringlit_3 : ident := 107%positive.
+Definition ___stringlit_4 : ident := 108%positive.
+Definition ___stringlit_5 : ident := 109%positive.
+Definition __l : ident := 93%positive.
+Definition _acquire : ident := 67%positive.
+Definition _b : ident := 79%positive.
+Definition _delete : ident := 104%positive.
+Definition _exit : ident := 62%positive.
+Definition _free : ident := 63%positive.
+Definition _freelock : ident := 66%positive.
+Definition _insert : ident := 88%positive.
 Definition _key : ident := 1%positive.
-Definition _l : ident := 70%positive.
-Definition _l1 : ident := 82%positive.
-Definition _l2 : ident := 83%positive.
-Definition _l_old : ident := 87%positive.
-Definition _l_old__1 : ident := 88%positive.
+Definition _l : ident := 73%positive.
+Definition _l1 : ident := 85%positive.
+Definition _l2 : ident := 86%positive.
+Definition _l_old : ident := 90%positive.
+Definition _l_old__1 : ident := 91%positive.
 Definition _left : ident := 4%positive.
 Definition _lock : ident := 8%positive.
-Definition _lookup : ident := 89%positive.
-Definition _lp : ident := 98%positive.
-Definition _lq : ident := 99%positive.
-Definition _main : ident := 107%positive.
-Definition _makelock : ident := 64%positive.
-Definition _malloc : ident := 63%positive.
-Definition _mid : ident := 93%positive.
-Definition _newt : ident := 69%positive.
-Definition _p : ident := 68%positive.
-Definition _p1 : ident := 80%positive.
-Definition _p2 : ident := 81%positive.
-Definition _pa : ident := 73%positive.
-Definition _pb : ident := 74%positive.
+Definition _lookup : ident := 92%positive.
+Definition _lp : ident := 101%positive.
+Definition _lq : ident := 102%positive.
+Definition _main : ident := 110%positive.
+Definition _makelock : ident := 65%positive.
+Definition _malloc : ident := 64%positive.
+Definition _mid : ident := 96%positive.
+Definition _n : ident := 69%positive.
+Definition _newt : ident := 72%positive.
+Definition _p : ident := 70%positive.
+Definition _p1 : ident := 83%positive.
+Definition _p2 : ident := 84%positive.
+Definition _pa : ident := 76%positive.
+Definition _pb : ident := 77%positive.
 Definition _printf : ident := 61%positive.
-Definition _pushdown_left : ident := 100%positive.
-Definition _q : ident := 96%positive.
-Definition _r : ident := 94%positive.
-Definition _release : ident := 67%positive.
+Definition _pushdown_left : ident := 103%positive.
+Definition _q : ident := 99%positive.
+Definition _r : ident := 97%positive.
+Definition _release : ident := 68%positive.
 Definition _right : ident := 5%positive.
+Definition _surely_malloc : ident := 71%positive.
 Definition _t : ident := 7%positive.
-Definition _tgl : ident := 91%positive.
-Definition _tgp : ident := 72%positive.
-Definition _tgq : ident := 97%positive.
-Definition _tgr : ident := 92%positive.
-Definition _tgt : ident := 79%positive.
+Definition _tgl : ident := 94%positive.
+Definition _tgp : ident := 75%positive.
+Definition _tgq : ident := 100%positive.
+Definition _tgr : ident := 95%positive.
+Definition _tgt : ident := 82%positive.
 Definition _tree : ident := 6%positive.
-Definition _tree_free : ident := 75%positive.
+Definition _tree_free : ident := 78%positive.
 Definition _tree_t : ident := 3%positive.
-Definition _treebox_free : ident := 77%positive.
-Definition _treebox_new : ident := 71%positive.
-Definition _turn_left : ident := 95%positive.
-Definition _v : ident := 86%positive.
+Definition _treebox_free : ident := 80%positive.
+Definition _treebox_new : ident := 74%positive.
+Definition _turn_left : ident := 98%positive.
+Definition _v : ident := 89%positive.
 Definition _value : ident := 2%positive.
-Definition _x : ident := 78%positive.
-Definition _y : ident := 84%positive.
-Definition _t'1 : ident := 108%positive.
-Definition _t'2 : ident := 109%positive.
-Definition _t'3 : ident := 110%positive.
-Definition _t'4 : ident := 111%positive.
-Definition _t'5 : ident := 112%positive.
+Definition _x : ident := 81%positive.
+Definition _y : ident := 87%positive.
+Definition _t'1 : ident := 111%positive.
+Definition _t'2 : ident := 112%positive.
+Definition _t'3 : ident := 113%positive.
+Definition _t'4 : ident := 114%positive.
+Definition _t'5 : ident := 115%positive.
 
 Definition v___stringlit_3 := {|
   gvar_info := (tarray tschar 5);
@@ -170,6 +173,27 @@ Definition v___stringlit_5 := {|
   gvar_volatile := false
 |}.
 
+Definition f_surely_malloc := {|
+  fn_return := (tptr tvoid);
+  fn_callconv := cc_default;
+  fn_params := ((_n, tuint) :: nil);
+  fn_vars := nil;
+  fn_temps := ((_p, (tptr tvoid)) :: (_t'1, (tptr tvoid)) :: nil);
+  fn_body :=
+(Ssequence
+  (Ssequence
+    (Scall (Some _t'1)
+      (Evar _malloc (Tfunction (Tcons tuint Tnil) (tptr tvoid) cc_default))
+      ((Etempvar _n tuint) :: nil))
+    (Sset _p (Etempvar _t'1 (tptr tvoid))))
+  (Ssequence
+    (Sifthenelse (Eunop Onotbool (Etempvar _p (tptr tvoid)) tint)
+      (Scall None (Evar _exit (Tfunction (Tcons tint Tnil) tvoid cc_default))
+        ((Econst_int (Int.repr 1) tint) :: nil))
+      Sskip)
+    (Sreturn (Some (Etempvar _p (tptr tvoid))))))
+|}.
+
 Definition f_treebox_new := {|
   fn_return := (tptr (tptr (Tstruct _tree_t noattr)));
   fn_callconv := cc_default;
@@ -184,7 +208,8 @@ Definition f_treebox_new := {|
 (Ssequence
   (Ssequence
     (Scall (Some _t'1)
-      (Evar _malloc (Tfunction (Tcons tuint Tnil) (tptr tvoid) cc_default))
+      (Evar _surely_malloc (Tfunction (Tcons tuint Tnil) (tptr tvoid)
+                             cc_default))
       ((Esizeof (tptr (Tstruct _tree_t noattr)) tuint) :: nil))
     (Sset _p
       (Ecast (Etempvar _t'1 (tptr tvoid))
@@ -192,7 +217,8 @@ Definition f_treebox_new := {|
   (Ssequence
     (Ssequence
       (Scall (Some _t'2)
-        (Evar _malloc (Tfunction (Tcons tuint Tnil) (tptr tvoid) cc_default))
+        (Evar _surely_malloc (Tfunction (Tcons tuint Tnil) (tptr tvoid)
+                               cc_default))
         ((Esizeof (Tstruct _tree_t noattr) tuint) :: nil))
       (Sset _newt
         (Ecast (Etempvar _t'2 (tptr tvoid)) (tptr (Tstruct _tree_t noattr)))))
@@ -204,8 +230,8 @@ Definition f_treebox_new := {|
       (Ssequence
         (Ssequence
           (Scall (Some _t'3)
-            (Evar _malloc (Tfunction (Tcons tuint Tnil) (tptr tvoid)
-                            cc_default))
+            (Evar _surely_malloc (Tfunction (Tcons tuint Tnil) (tptr tvoid)
+                                   cc_default))
             ((Esizeof (tarray (tptr tvoid) 2) tuint) :: nil))
           (Sset _l
             (Ecast (Etempvar _t'3 (tptr tvoid))
@@ -367,8 +393,8 @@ Definition f_insert := {|
               (Ssequence
                 (Ssequence
                   (Scall (Some _t'1)
-                    (Evar _malloc (Tfunction (Tcons tuint Tnil) (tptr tvoid)
-                                    cc_default))
+                    (Evar _surely_malloc (Tfunction (Tcons tuint Tnil)
+                                           (tptr tvoid) cc_default))
                     ((Esizeof (Tstruct _tree_t noattr) tuint) :: nil))
                   (Sset _p1
                     (Ecast (Etempvar _t'1 (tptr tvoid))
@@ -376,8 +402,8 @@ Definition f_insert := {|
                 (Ssequence
                   (Ssequence
                     (Scall (Some _t'2)
-                      (Evar _malloc (Tfunction (Tcons tuint Tnil)
-                                      (tptr tvoid) cc_default))
+                      (Evar _surely_malloc (Tfunction (Tcons tuint Tnil)
+                                             (tptr tvoid) cc_default))
                       ((Esizeof (Tstruct _tree_t noattr) tuint) :: nil))
                     (Sset _p2
                       (Ecast (Etempvar _t'2 (tptr tvoid))
@@ -401,8 +427,9 @@ Definition f_insert := {|
                       (Ssequence
                         (Ssequence
                           (Scall (Some _t'3)
-                            (Evar _malloc (Tfunction (Tcons tuint Tnil)
-                                            (tptr tvoid) cc_default))
+                            (Evar _surely_malloc (Tfunction
+                                                   (Tcons tuint Tnil)
+                                                   (tptr tvoid) cc_default))
                             ((Esizeof (tarray (tptr tvoid) 2) tuint) :: nil))
                           (Sset _l1
                             (Ecast (Etempvar _t'3 (tptr tvoid))
@@ -432,9 +459,10 @@ Definition f_insert := {|
                               (Ssequence
                                 (Ssequence
                                   (Scall (Some _t'4)
-                                    (Evar _malloc (Tfunction
-                                                    (Tcons tuint Tnil)
-                                                    (tptr tvoid) cc_default))
+                                    (Evar _surely_malloc (Tfunction
+                                                           (Tcons tuint Tnil)
+                                                           (tptr tvoid)
+                                                           cc_default))
                                     ((Esizeof (tarray (tptr tvoid) 2) tuint) ::
                                      nil))
                                   (Sset _l2
@@ -467,11 +495,12 @@ Definition f_insert := {|
                                       (Ssequence
                                         (Ssequence
                                           (Scall (Some _t'5)
-                                            (Evar _malloc (Tfunction
-                                                            (Tcons tuint
-                                                              Tnil)
-                                                            (tptr tvoid)
-                                                            cc_default))
+                                            (Evar _surely_malloc (Tfunction
+                                                                   (Tcons
+                                                                    tuint
+                                                                    Tnil)
+                                                                   (tptr tvoid)
+                                                                   cc_default))
                                             ((Esizeof (Tstruct _tree noattr) tuint) ::
                                              nil))
                                           (Sset _p
@@ -1348,6 +1377,10 @@ Definition global_definitions : list (ident * globdef fundef type) :=
                      {|cc_vararg:=true; cc_unproto:=false; cc_structret:=false|}))
      (Tcons (tptr tschar) Tnil) tint
      {|cc_vararg:=true; cc_unproto:=false; cc_structret:=false|})) ::
+ (_exit,
+   Gfun(External (EF_external "exit"
+                   (mksignature (AST.Tint :: nil) None cc_default))
+     (Tcons tint Tnil) tvoid cc_default)) ::
  (_free, Gfun(External EF_free (Tcons (tptr tvoid) Tnil) tvoid cc_default)) ::
  (_malloc,
    Gfun(External EF_malloc (Tcons tuint Tnil) (tptr tvoid) cc_default)) ::
@@ -1367,6 +1400,7 @@ Definition global_definitions : list (ident * globdef fundef type) :=
    Gfun(External (EF_external "release"
                    (mksignature (AST.Tint :: nil) None cc_default))
      (Tcons (tptr tvoid) Tnil) tvoid cc_default)) ::
+ (_surely_malloc, Gfun(Internal f_surely_malloc)) ::
  (_treebox_new, Gfun(Internal f_treebox_new)) ::
  (_tree_free, Gfun(Internal f_tree_free)) ::
  (_treebox_free, Gfun(Internal f_treebox_free)) ::
@@ -1377,26 +1411,27 @@ Definition global_definitions : list (ident * globdef fundef type) :=
 
 Definition public_idents : list ident :=
 (_main :: _delete :: _pushdown_left :: _turn_left :: _lookup :: _insert ::
- _treebox_free :: _tree_free :: _treebox_new :: _release :: _acquire ::
- _freelock :: _makelock :: _malloc :: _free :: _printf :: ___builtin_debug ::
- ___builtin_nop :: ___builtin_write32_reversed ::
- ___builtin_write16_reversed :: ___builtin_read32_reversed ::
- ___builtin_read16_reversed :: ___builtin_fnmsub :: ___builtin_fnmadd ::
- ___builtin_fmsub :: ___builtin_fmadd :: ___builtin_fmin ::
- ___builtin_fmax :: ___builtin_ctzll :: ___builtin_ctzl :: ___builtin_ctz ::
- ___builtin_clzll :: ___builtin_clzl :: ___builtin_clz ::
- ___builtin_bswap64 :: ___compcert_i64_umulh :: ___compcert_i64_smulh ::
- ___compcert_i64_sar :: ___compcert_i64_shr :: ___compcert_i64_shl ::
- ___compcert_i64_umod :: ___compcert_i64_smod :: ___compcert_i64_udiv ::
- ___compcert_i64_sdiv :: ___compcert_i64_utof :: ___compcert_i64_stof ::
- ___compcert_i64_utod :: ___compcert_i64_stod :: ___compcert_i64_dtou ::
- ___compcert_i64_dtos :: ___compcert_va_composite ::
- ___compcert_va_float64 :: ___compcert_va_int64 :: ___compcert_va_int32 ::
- ___builtin_va_end :: ___builtin_va_copy :: ___builtin_va_arg ::
- ___builtin_va_start :: ___builtin_membar :: ___builtin_annot_intval ::
- ___builtin_annot :: ___builtin_memcpy_aligned :: ___builtin_fsqrt ::
- ___builtin_fabs :: ___builtin_bswap16 :: ___builtin_bswap32 ::
- ___builtin_bswap :: ___builtin_ais_annot :: nil).
+ _treebox_free :: _tree_free :: _treebox_new :: _surely_malloc :: _release ::
+ _acquire :: _freelock :: _makelock :: _malloc :: _free :: _exit ::
+ _printf :: ___builtin_debug :: ___builtin_nop ::
+ ___builtin_write32_reversed :: ___builtin_write16_reversed ::
+ ___builtin_read32_reversed :: ___builtin_read16_reversed ::
+ ___builtin_fnmsub :: ___builtin_fnmadd :: ___builtin_fmsub ::
+ ___builtin_fmadd :: ___builtin_fmin :: ___builtin_fmax ::
+ ___builtin_ctzll :: ___builtin_ctzl :: ___builtin_ctz :: ___builtin_clzll ::
+ ___builtin_clzl :: ___builtin_clz :: ___builtin_bswap64 ::
+ ___compcert_i64_umulh :: ___compcert_i64_smulh :: ___compcert_i64_sar ::
+ ___compcert_i64_shr :: ___compcert_i64_shl :: ___compcert_i64_umod ::
+ ___compcert_i64_smod :: ___compcert_i64_udiv :: ___compcert_i64_sdiv ::
+ ___compcert_i64_utof :: ___compcert_i64_stof :: ___compcert_i64_utod ::
+ ___compcert_i64_stod :: ___compcert_i64_dtou :: ___compcert_i64_dtos ::
+ ___compcert_va_composite :: ___compcert_va_float64 ::
+ ___compcert_va_int64 :: ___compcert_va_int32 :: ___builtin_va_end ::
+ ___builtin_va_copy :: ___builtin_va_arg :: ___builtin_va_start ::
+ ___builtin_membar :: ___builtin_annot_intval :: ___builtin_annot ::
+ ___builtin_memcpy_aligned :: ___builtin_fsqrt :: ___builtin_fabs ::
+ ___builtin_bswap16 :: ___builtin_bswap32 :: ___builtin_bswap ::
+ ___builtin_ais_annot :: nil).
 
 Definition prog : Clight.program := 
   mkprogram composites global_definitions public_idents _main Logic.I.
